\section*{Занятие 9}
\begin{exercise}[1]
	\begin{table}
		\centering
		\begin{tabular}{|c|c|c|c|}
			\hline
			$X$ & $Y$ & $Z$ & $P$ \\ \hline
			$2$ & $4$ & $6$ & $0,3 \cdot 0,4 = 0,12$ \\ \hline
			2 & 5 & 7 & \multirow{2}{*}{$0,3 \cdot 0,4 + 0,7 \cdot 0,4 = 0,46$} \\ \cline{1-3}
			3 & 4 & 7 & \\ \hline
			3 & 5 & 8 & $0,7 \cdot 0,6 = 0,42$ \\ \hline 
		\end{tabular}
		\begin{tabular}{|c|ccc|}
			\hline
			$Z$ & 6 & 7 & 8 \\ \hline
			$P$ & 0,12 & 0,46 & 0,42 \\ \hline
		\end{tabular}
	\caption{Занятие 9 - упражение 1}
	\end{table}
	$\Rightarrow M(Z) = 6 \cdot 0,12 + 7 \cdot 0,46 + 8 \cdot 0,42 = 7,3$
\end{exercise}

\begin{exercise}[2]
	$f(x) = \begin{cases}
		\lambda e^{-\lambda x} \text{ при } x \geq 0 \\
		0 \text{ при } x < 0
	\end{cases}$ \\
	$Z = X+Y \Rightarrow f(z) = \int_{-\infty}^{+\infty}f_1(x) f_2(z-x)\,dx$ \\
	При $z \geq 0 \Rightarrow f(z) = \int_{0}^{z}\lambda e^{-\lambda x} \cdot \lambda e^{-\lambda (z-x)}\,dx = \int_{0}^{z}\lambda^2 e^{-\lambda z}\,dx = \lambda^2 e^{-\lambda z}$ \\
	При $z < 0$, $f(z)=0$
\end{exercise}

\begin{exercise}[3]
	$Z=2X-Y+5$, $M(X)=3$, $M(Y)=5$, $D(X)=2$, $D(Y)=1$ \\
	$M(Z)=2M(X)-M(Y)+5=6$ \\
	$D(Z)=D(2X)+D(Y)=4D(X)+D(Y)=9=\sigma^2 \Rightarrow \sigma=3$
\end{exercise}

\begin{exercise}[4]
	$X$ и $Y$ независимы. $f_1(x) = f_2(y) = \frac{1}{2}$. $X, Y ~ U(0, 2)$. $Z=X+Y$ \\
	При $0 \leq z < 2$, $f(z) = \int_{0}^{z}\frac{1}{2} \cdot \frac{1}{2}\,dx = \frac{z}{4}$ \\
	При $2 \leq z < 4$, $f(z) = \int_{z-2}^{2}\frac{1}{2} \cdot \frac{1}{2}\,dx = \frac{1}{4}(2-z+2) = 1-0,25z$ \\
	При остальных $z$, $f(z)=0$
\end{exercise}

\begin{exercise}[6]
	Св $X$ и $Y$ независимы, равномерно на $(0, 1)$. $Z=Y/X^2$
	
	 У нас есть $F(z) = P(Z \leq z) = P(Y/X^2 \leq z)$, $y/x^2\leq z \Leftrightarrow y \leq zx^2$
	 \begin{itemize}
	 	\item При $z \leq 0$, $f(z)=0$
	 	\item При $0 < z \leq 1$, $F(z) = \int_{0}^{1}\,dx\int_{0}^{zx^2}\,dy = \int_{0}^{1}zx^2\,dx = \frac{z}{3}$ \\ $\Rightarrow f(z) = \frac{1}{3}$
	 	\item При $z > 1$, $y \leq zx^2 \Rightarrow x \geq \sqrt{\frac{y}{z}}$ \\ $\Rightarrow F(z) = \int_{0}^{1}\,dy \int_{\sqrt{y/z}}^{1}\,dx = \int_{0}^{1}(1 - \sqrt{\frac{y}{z}})\,dy=1-\frac{2}{3\sqrt{z}}$ \\ $\Rightarrow f(z) = 1/(3z^{1,5})$
	 \end{itemize}
\end{exercise}

\begin{exercise}[7]
	\textbf{$U=min(X, Y)$}
	\begin{itemize}
		\item При $u < 0$, $F(u)=0$
		\item При $0 \leq u < 1$, $F(u) = P(min(X, Y) \leq u) = 1 - P(min(X, Y) > u) = 1 - \int_{u}^{1}\int_{u}^{1}\,dx\,dy = 2u-u^2$
		\item При $u>1$, $F(u)=1$
	\end{itemize}
	$\Rightarrow M(U) = \int_{0}^{1}u(2-2u)\,du=1/3$ \\
	$\Rightarrow D(U) = \int_{0}^{1}(u-\frac{1}{3})^2(2-2u)\,du = 1/18$
	
	\textbf{$V=max(X, Y)$}
	\begin{itemize}
		\item При $v < 0$, $F(v) = 0$
		\item При $0 \leq v < 1$, $F(v) = P(max(X, Y) \leq v) = \int_{0}^{v}\int_{0}^{v}\,dx\,dy = v^2 \Rightarrow f(v) = 2v$
		\item При $v > 1$, $F(v)=1$
	\end{itemize}
	$\Rightarrow M(v) = \int_{0}^{1}v\cdot 2v\,dv = 2/3$ \\
	$\Rightarrow D(v) = \int_{0}^{1}(v-\frac{2}{3})^2\cdot 2v\,dv = 1/18$
\end{exercise}

\begin{exercise}[9]
	Площадь треугольника $ABC$ равна 1 $\Rightarrow f(x, y) = 1$ \\ $y \leq \frac{x}{2} \Rightarrow \begin{cases}
		0 \leq y \leq \frac{x}{2} \\ 2y \leq x \leq 2
	\end{cases}$ \\ $f_1(x) = \int_{0}^{x/2}1\,dy = \frac{2}{x}$ \\ $f_2(y) = \int_{2y}^{2}1\,dx = 2-2y$ \\ $M(X) = \int_{0}^{2}x \cdot \frac{x}{2}\,dx = \frac{4}{3}$, $M(X^2) = \int_{0}^{2}x^2 \cdot \frac{x}{2}\,dx = 2$ \\ $M(Y) = \int_{0}^{1}y(2-2y)\,dy = \frac{1}{3}$,  $M(Y^2) = \int_{0}^{1}y^2(2-2y)\,dy=\frac{1}{6}$ \\ $M(\overset{\circ}{X}\cdot \overset{\circ}{Y}) = \int_{0}^{2}\,dx\int_{0}^{x/2}(x-\frac{4}{3})(y-\frac{1}{3})\,dy = \cdots = \frac{1}{18}$ \\ $\sigma_x^2 = M(X^2)-M(X)^2=2-\frac{16}{9}=\frac{2}{9}$ \\ $\sigma_y^2 = M(Y^2)-M(Y)^2=\frac{1}{6} - \frac{1}{9} = \frac{1}{18}$ \\ $\Rightarrow r_{xy} = \frac{1}{2}$

	Линия регрессии: $\frac{y-1/3}{\sigma_y} = r_{xy}\frac{x-4/3}{\sigma_x} \Rightarrow y = \frac{x}{4}$
\end{exercise}

\begin{exercise}[11]
	$f(x) \rightarrow g(y)$, $Y = min(X, X^2)$. У нас есть
	\begin{itemize}
		\item При $x<0$ или $x \geq 1$, $min(X, X^2)=X$
		\item При $0 \leq x < 1$, $min(X, X^2)=X^2$
	\end{itemize}
	$G(y) = P(Y \leq y) = P(min(X, X^2) \leq y)$
	\begin{itemize}
		\item При $y < 0$, $G(y) = P(X \leq y) = \int_{-\infty}^{y}f(x)\,dx = F(y) \Rightarrow g(y)=f(y)$
		\item При $0 \leq y < 1$, $G(y) = P(X^2 \leq y) = P(X \leq \sqrt{Y}) = \int_{0}^{\sqrt{y}}f(x)\,dx = F(\sqrt{y}) \Rightarrow g(y) = f(\sqrt{y})(\sqrt{y})'=\frac{f(\sqrt{y})}{2\sqrt{y}}$
		\item При $y \geq 1$, $G(y) = P(X \leq y) = \int_{1}^{y}f(x)\,dx = F(y) \Rightarrow g(y)=f(y)$
	\end{itemize}
\end{exercise}

\begin{exercise}[12]
	$X_1, X_2 \rightarrow f(x_1, x_2) = \frac{2}{\pi^2(x_1^2+1)(x_2^2+4)}$, $g(y_1, y_2) \rightarrow Y_1, Y_2$, $X_1 = \tg(Y_1)$, $X_2 = 2\tg(Y_2)$, $|Y_1|<\pi/2$, $|Y_2|<\pi/2$
	
	При $|y_1| < \pi/2$, $|y_2| < \pi/2$
	\begin{align*}
		G(y_1, y_2) & = P(Y_1 \leq y_1, Y_2 \leq y_2) \\
		& P(\arctg(X_1) \leq y_1, \arctg(\frac{X_2}{2}) \leq y_2) \\ & P(X_1 \leq \tg(y_1), X_2 \leq 2\tg(y_2)) \\ & \int_{-\infty}^{\tg y_1}\int_{-\infty}^{2\tg y_2}\frac{2\,dx_1\,dx_2}{\pi^2(x_1^2+1)(x_2^2+4)} \\ & \int_{-\infty}^{\tg y_1}\,dx_1\cdot \frac{2}{\pi^2(x_1^2+1)} \cdot \frac{1}{2} \arctg(\frac{x_2}{2})\Big|^{2\tg y_2}_{-\infty} \\ & \int_{-\infty}^{\tg y_1}(y_2 + \frac{\pi}{2})\frac{\,dx_1}{\pi^2(x_1^2+1)} \\ & \frac{1}{\pi^2}(y_1+\frac{\pi}{2})(y_2 + \frac{\pi}{2})
	\end{align*}
	$\Rightarrow g(y_1, y_2) = \frac{\partial^2G(y_1, y_2)}{\partial y_1 \partial y_2} = \frac{1}{\pi^2}$
	
	При остальных $y_1$, $y_2$, $g(y_1, y_2) = 0$
\end{exercise}