\chapter*{Chapter 7}

\begin{exer}[7.7]
	\begin{figure}[h]
		\includegraphics[width=\textwidth]{exercise-7-7.png}
		\caption{Exercise 7.7 - Fundamental domain of $L$}
	\end{figure}
	$\det (L) = \Vol (\mathcal{F})$
\end{exer}

\begin{exer}[7.43] $t = b_1 b_2 / \lVert b_1 \rVert^2$ and $b_2^* = b_2 - tb_1$ \\ $\Rightarrow b_2^* \cdot b_1 = b_1 (b_2 - tb_1) = b_1 b_2 - t \lVert b_1 \rVert^2 = b_1 b_2 - \frac{b_1 b_2}{\lVert b_1 \rVert^2} \cdot \lVert b_1 \rVert^2 = 0$ \\ Hence $b_2^* \perp b_1$ and $b_2^*$ is the projection of $b_2$ onto the orthogonal complement of $b_1$
\end{exer}

\begin{exer}[7.44]
	\begin{enumerate}
		\item [(a)] $\lVert a - tb \rVert^2 = (a - tb)^2 = a^2 - 2abt + t^2b^2 = \lVert a\rVert^2 + t^2 \lVert b\rVert^2 - 2abt \geq 0$ \\ $\Leftrightarrow a - tb = 0 \Rightarrow t = \frac{ab}{\lVert b \rVert^2}$
		\item [(b)] 0
		\item [(c)] $(a - tb)\cdot b = ab - t \lVert b \rVert^2 = ab - \frac{ab}{\lVert b \rVert^2} \cdot \lVert b \rVert^2 = 0$. \\ Therefore $a - tb$ is the projection of $a$ onto the orthogonal complement of $b$
	\end{enumerate}
\end{exer}

\begin{exer}[7.45]
	\begin{algorithm}
		\While{True}{
		\If{$\lVert v_2 \rVert < \lVert v_1 \rVert$}{swap $v_1$ and $v_2$}
		$m \gets \nint{v_1 \cdot v_2 / \lVert v_1 \rVert^2}$\;
		\If{$m = 0$}{return $(v_1, v_2)$}
		Replace $v_2$ with $v_2 - mv_1$
	}
	\TitleOfAlgo{Gauss's latice reduction algorithm}
	\end{algorithm}
	\begin{enumerate}
		\item [(a)] $v_1 = (14, -47)$, $v_2 = (-362, -131)$, 6 steps
		\item [(b)] $v_1 = (14, -47)$, $v_2 = (-362, -131)$, 6 steps
		\item [(c)] $v_1 = (147, 330)$, $v_2 = (690, -207)$, 7 steps
	\end{enumerate}
\end{exer}

\begin{exer}[7.46]
	\begin{enumerate}
		\item [(a)] $W^\perp$ is the orthogonal complement of $W$ in $V$ $\Rightarrow \vec{z} \in W^\perp$, $\vec{z}\cdot\vec{y} = 0, \forall \vec{y} \in W$ \\ With $\vec{z_1}, \vec{z_2} \in W^\perp \Rightarrow \vec{z_1}\cdot\vec{y} = \vec{z_2}\cdot\vec{y} = 0, \forall \vec{y} \in W$ \\ $\Rightarrow (\vec{z_1} + \vec{z_2})\cdot\vec{y} = 0 \Rightarrow \vec{z_1} + \vec{z_2} \in W^\perp$ \\ $\alpha\vec{z_1}\cdot\vec{y} = \alpha \cdot 0 = 0 \Rightarrow \alpha\vec{z_1} \in W^\perp, \forall \alpha \in \mathbb{R}$
		\item [(b)] We have 2 methods
		\begin{itemize}
			\item \textit{First method}: Show that $W \cup W^\perp = \{\vec{0}\}$. If $\vec{u}$ belongs to both $W$ and $W^\perp$, then $<u, u> = 0 \Rightarrow \vec{u} = \vec{0}$.
			
			Now denote $U = W + W^\perp$, we prove that $W = V$. We can choose an orthonormal basis in $U$ and extend it to orthonormal basis in $V$. Thus, if $U \neq V$, there is an element $\vec{e}$ in the basis of $V$ orthonormal to $U$. Since $U$ contains $W$, $e$ is orthonormal to $U \Rightarrow \vec{e} \in W^\perp$. The latter is a subspace of $W$, therefore $e$ is in $W$, which is contrary.
			\item \textit{Second method}: Let $\{e_1, e_2, \cdots, e_k\}$ be an orthonormal basis of the subspace $W$. For each $v \in V$, let $$P(v) = \sum_{j=1}^{k} <v, e_j> e_j$$ $$\Rightarrow (\forall v \in V): v = \underbrace{P(v)}_{\in W} + \underbrace{(v - P(v))}_{\in W^\perp}$$
			The fact that $v - P(v) \in W^\perp$ is: \\ if $j \in \{1, 2, \cdots, k\}$ then $$<v-P(v), e_j> = <v - \sum_{l=1}^{k}<v, e_l>e_l, e_j> = <v, e_j> - <v, e_j> = 0$$
			Since $\{e_1, \cdots, e_k\}$ is a basic of $W$, this prove that $v-P(v) \in W^\perp$
		\end{itemize}
		\item [(c)] $\lVert v \rVert^2 = <v, v> = (aw + bw')^2 = a^2w^2 + 2abww' + b^2w'^2 = a^2 \lVert w \rVert^2 + 0 + b^2 \lVert w' \rVert^2 = a^2 \lVert w \rVert^2 + b^2 \lvert w' \rVert^2$
	\end{enumerate}
\end{exer}